theorems/experiments/ir/opt/Reify.lean
@@ -81,4 +81,7 @@ where
     /- these are definitionally equal, so it's fine anyway and IR.eval is on the outside -/
     let proof := mkApp7 congrLemmaQ nQ lhsExpr rhsExpr lhsEval rhsEval lhsProof rhsProof
 
+    let actualType ← mkEq (← M.mkEvalIR idx ξQ σQ irExpr) body
+    let proof := mkExpectedPropHint proof actualType
+
     return ⟨ir, irExpr, body, pure proof⟩
